theories/aneris_lang/resources.v
@@ -1,12 +1,11 @@
-From iris.algebra Require Import auth gmap frac agree coPset gset frac_auth ofe.
-From iris.base_logic Require Export own gen_heap.
-From iris.bi.lib Require Import fractional.
-From iris.base_logic.lib Require Import viewshifts saved_prop gen_heap.
-From iris.program_logic Require Export weakestpre.
-From iris.program_logic Require Import ectx_lifting total_ectx_lifting.
-From iris.proofmode Require Import tactics.
-From aneris.aneris_lang Require Export helpers aneris_lang notation tactics network.
 From stdpp Require Import fin_maps gmap.
+From iris.algebra Require Import auth gmap frac agree coPset gset frac_auth ofe.
+From iris.bi.lib Require Import fractional.
+From iris.base_logic.lib Require Import viewshifts saved_prop.
+From iris.program_logic Require Import ectx_lifting.
+From iris.proofmode Require Import tactics.
+From aneris.program_logic Require Import gen_heap_light.
+From aneris.aneris_lang Require Export aneris_lang notation network.
 From RecordUpdate Require Import RecordSet.
 Set Default Proof Using "Type".
 
@@ -16,473 +15,492 @@ Import RecordSetNotations.
 
 Record node_gnames := Node_gname {
   heap_name : gname;
-  heap_meta_name : gname;
-  socket_name : gname;
-  socket_meta_name : gname;
+  sockets_name : gname;
 }.
 
-Definition node_gnamesO := leibnizO node_gnames.
-Definition system_state_mapUR : ucmraT := gmapUR ip_address (agreeR node_gnamesO).
-
-Definition socket_interpR : cmraT :=
-  authR (gmapUR socket_address (agreeR (leibnizO gname))).
+(** CMRA shorthands *)
+Definition node_gnamesO :=
+  leibnizO node_gnames.
+Definition node_gnames_mapUR : ucmraT :=
+  gmapUR ip_address (agreeR node_gnamesO).
+Definition local_heapUR : ucmraT :=
+  gen_heapUR loc base_lang.val.
+Definition local_socketsUR : ucmraT :=
+  gen_heapUR socket_handle (socket * message_soup * message_soup).
+Definition socket_interpUR : ucmraT :=
+  gmapUR socket_address (agreeR (leibnizO gname)).
 
 Instance system_state_mapUR_unit : Unit (gmap ip_address (agree node_gnames)) :=
   (∅ : gmap ip_address (agree node_gnames)).
-Global Instance system_state_core_id (x : system_state_mapUR) : CoreId x.
+Global Instance system_state_core_id (x : node_gnames_mapUR) : CoreId x.
 Proof. apply _. Qed.
 
 Definition socket_interp Σ := message -d> iPropO Σ.
 
-(** The system CMRA. *)
-Class distG Σ := DistG {
-  dist_invG :> invG Σ;
-  dist_mapG :> inG Σ (authR system_state_mapUR);
-  dist_map_name : gname;
-  dist_heapG :> gen_heapPreG loc ground_lang.val Σ;
-  (* network *)
-  dist_socketG :> gen_heapPreG socket_handle (socket * message_soup * message_soup) Σ;
-  dist_freeipsG :> inG Σ (authUR (gset_disjUR ip_address));
-  dist_freeips_name : gname;
-  dist_freeportsG :> inG Σ (authUR (gmapUR ip_address (gset_disjUR port)));
-  dist_freeports_name : gname;
-  dist_siG :> inG Σ socket_interpR;
-  dist_si_name : gname;
-  dist_fixedG :> inG Σ (agreeR (gsetUR socket_address));
-  dist_fixed_name : gname;
-  dist_savedPredG :> savedPredG Σ message;
+(** The system CMRA *)
+Class anerisG Σ := AnerisG {
+  aneris_invG :> invG Σ;
+  (* global tracking of the ghost names of node-local heaps *)
+  aneris_node_gnames_mapG :> inG Σ (authR node_gnames_mapUR);
+  aneris_node_gnames_name : gname;
+  (* local heap *)
+  aneris_heapG :> inG Σ (authR local_heapUR);
+  (* local sockets *)
+  aneris_socketG :> inG Σ (authR local_socketsUR);
+  (* free ips *)
+  aneris_freeipsG :> inG Σ (authUR (gset_disjUR ip_address));
+  aneris_freeips_name : gname;
+  (* free ports  *)
+  aneris_freeportsG :> inG Σ (authUR (gmapUR ip_address (gset_disjUR port)));
+  aneris_freeports_name : gname;
+  (* socket interpretations *)
+  aneris_siG :> inG Σ (authR socket_interpUR);
+  aneris_savedPredG :> savedPredG Σ message;
+  aneris_si_name : gname;
+  (* socket addresses with fixed socket interpretations *)
+  aneris_fixedG :> inG Σ (agreeR (gsetUR socket_address));
+  aneris_fixed_name : gname;
 }.
 
-Arguments gen_heap_name {_ _ _ _ _} _ : assert.
-Arguments gen_meta_name {_ _ _ _ _} _ : assert.
+Class anerisPreG Σ := AnerisPreG {
+  anerisPre_invG :> invPreG Σ;
+  anerisPre_node_gnames_mapG :> inG Σ (authR node_gnames_mapUR);
+  anerisPre_heapG :> inG Σ (authR local_heapUR);
+  anerisPre_socketG :> inG Σ (authR local_socketsUR);
+  anerisPre_freeipsG :> inG Σ (authUR (gset_disjUR ip_address));
+  anerisPre_freeportsG :> inG Σ (authUR (gmapUR ip_address (gset_disjUR port)));
+  anerisPre_siG :> inG Σ (authR socket_interpUR);
+  anerisPre_savedPredG :> savedPredG Σ message;
+  anerisPre_fixedG :> inG Σ (agreeR (gsetUR socket_address));
+}.
 
-Definition gen_heap_loc_instance γ γ' `{distG Σ} :=
-  GenHeapG loc ground_lang.val _ _ _ _ _ _ γ γ'.
+Definition anerisΣ : gFunctors :=
+  #[invΣ;
+   GFunctor (authR node_gnames_mapUR);
+   GFunctor (authR local_heapUR);
+   GFunctor (authR local_socketsUR);
+   GFunctor (authUR (gset_disjUR ip_address));
+   GFunctor (authUR (gmapUR ip_address (gset_disjUR port)));
+   GFunctor (authR socket_interpUR);
+   savedPredΣ message;
+   GFunctor (agreeR (gsetUR socket_address))].
 
-Definition gen_heap_soc_instance γ γ' `{distG Σ} :=
-  GenHeapG socket_handle (socket * message_soup * message_soup) _ _ _ _ _ _ γ γ'.
+Global Instance subG_anerisPreG {Σ} : subG anerisΣ Σ → anerisPreG Σ.
+Proof. constructor; solve_inG. Qed.
 
-Section Definitions.
-  Context `{dG : distG Σ}.
+Section definitions.
+  Context `{aG : !anerisG Σ}.
 
-  Definition mapsto_node_def (ip : ip_address) (x : node_gnames) :=
-    own (dist_map_name) (◯ {[ ip := to_agree x ]} : auth system_state_mapUR).
+  (** Ghost names for node-local heaps *)
+  Definition node_gnames_auth (m : gmap ip_address node_gnames) :=
+     own (A := authR node_gnames_mapUR) aneris_node_gnames_name (● (to_agree <$> m)).
+
+  Definition mapsto_node_def (ip : ip_address) (γn : node_gnames) :=
+    own (aneris_node_gnames_name) (◯ {[ ip := to_agree γn ]}).
   Definition mapsto_node_aux : seal (@mapsto_node_def). by eexists. Qed.
   Definition mapsto_node := unseal mapsto_node_aux.
   Definition mapsto_node_eq : @mapsto_node = @mapsto_node_def :=
     seal_eq mapsto_node_aux.
 
-  Global Instance mapsto_node_persistent n x : Persistent (mapsto_node n x).
-  Proof. rewrite mapsto_node_eq /mapsto_node_def. apply _. Qed.
+  Definition is_node (ip : ip_address) := (∃ γn, mapsto_node ip γn)%I.
 
-  (** Ghost state for the heap of a given node *)
-  Definition mapsto_l n l q v :=
-    (∃ γ's, mapsto_node n γ's ∗
-            mapsto (hG := gen_heap_loc_instance
-                            (heap_name γ's)
-                            (heap_meta_name γ's)) l q v)%I.
+  (** Node-local heap *)
+  Definition heap_ctx (γn : node_gnames) (h : gmap loc base_lang.val) :=
+    gen_heap_light_ctx (heap_name γn) h.
 
-  (** Ghost state for the sockets of a given node *)
-  Definition mapsto_s n h q (s: socket * message_soup * message_soup) :=
-    (∃ γ's, mapsto_node n γ's ∗
-            mapsto (hG := gen_heap_soc_instance
-                            (socket_name γ's)
-                            (socket_meta_name γ's)) h q s)%I.
-End Definitions.
+  Definition mapsto_heap (ip : ip_address) (l : loc) (q : Qp)
+             (v : base_lang.val) :=
+    (∃ γn, mapsto_node ip γn ∗ lmapsto (heap_name γn) l q v)%I.
 
-Notation "n n↦ x" := (mapsto_node n x)
-                       (at level 20, format "n  n↦  x") : uPred_scope.
+  (** Sockets *)
+  Definition sockets_ctx (γn : node_gnames)
+             (s : gmap socket_handle (socket * message_soup * message_soup)) :=
+    gen_heap_light_ctx (sockets_name γn) s.
 
-Open Scope uPred_scope.
+  Definition mapsto_socket (ip : ip_address) (z : socket_handle) (q : Qp)
+             (s: socket * message_soup * message_soup) :=
+    (∃ γn, mapsto_node ip γn ∗ lmapsto (sockets_name γn) z q s)%I.
 
-(** Ghost state notations for heap and socket resources *)
+  (** Ghost names of saved socket interpretations *)
+  Definition saved_si_auth (sis : gmap socket_address gname) :=
+      own (A:=(authR socket_interpUR)) aneris_si_name (● (to_agree <$> sis)).
 
-(** Heaps n↦ *)
-Notation "l ↦[ n ]{ q } v" := (mapsto_l n l q v)
-  (at level 20, q at level 50, format "l  ↦[ n ]{ q }  v") : uPred_scope.
-Notation "l ↦[ n ] v" := (l ↦[n]{1} v)
-  (at level 20, format "l  ↦[ n ]  v") : uPred_scope.
-Notation "l ↦[ n ]{ q } -" := (∃ v, l ↦[n]{q} v)%I
-  (at level 20, q at level 50, format "l  ↦[ n ]{ q }  -") : uPred_scope.
-Notation "l ↦[ n ] -" := (l ↦[n]{1} -)%I
-  (at level 20, format "l  ↦[ n ]  -") : uPred_scope.
+  Definition saved_si (a : socket_address) (γ : gname) :=
+    own aneris_si_name (◯ {[ a := to_agree γ ]}).
 
-(** Sockets s↦ *)
-Notation "h s↦[ n ]{ q } z" := (mapsto_s n h q z)
-  (at level 20, q at level 50, format "h  s↦[ n ]{ q }  z") : uPred_scope.
-Notation "h s↦[ n ] z" := (mapsto_s n h 1 z) (at level 20) : uPred_scope.
+  (** Socket interpretation [Φ] of address [a] *)
+  Definition si_pred a (Φ : socket_interp Σ) : iProp Σ :=
+    (∃ γ, saved_si a γ ∗ saved_pred_own γ Φ)%I.
 
-(** Lookup stored socket interpretation γ↦ *)
-Notation "a γ↦ γ" :=
-  (own (A:=socket_interpR)
-       dist_si_name (◯ {[ a := (to_agree γ) ]})) (at level 20) : uPred_scope.
+  (** The set [A] of addresses with fixed socket interpretations *)
+  Definition fixed (A : gset socket_address) :=
+    own aneris_fixed_name (to_agree A).
 
-(* For some reason, Coq cannot find these RAs, so we define them explicitly *)
-Definition ownS γ (m : gmap ip_address node_gnames) `{distG Σ} :=
-  own (A := authR system_state_mapUR) γ (● (to_agree <$> m)).
+  (** Free ip addresses *)
+  Definition free_ips_auth (A : gset ip_address) :=
+    own aneris_freeips_name (● GSet A).
 
-Definition ownF (f : gset socket_address) `{distG} :=
-  own dist_fixed_name (to_agree f).
+  Definition free_ip (ip : ip_address) :=
+    own aneris_freeips_name (◯ GSet {[ ip ]}).
 
-Global Instance mapsto_n_timeless
-       `{distG Σ} (n : ip_address) v : Timeless (n n↦ v).
-Proof. rewrite mapsto_node_eq /mapsto_node_def. apply _. Qed.
+  (** Free ports *)
+  Definition free_ports_auth (P : gmap ip_address (gset_disjUR port)) :=
+    own aneris_freeports_name (● P).
 
-Global Instance mapsto_l_timeless
-       `{distG Σ} (n : ip_address) l q v : Timeless (mapsto_l n l q v).
-Proof.
-  rewrite /mapsto_l /Timeless.
-  iIntros ">H". iDestruct "H" as (γ's) "(H1 & H2)".
-  iExists γ's. iFrame.
-Qed.
+  Definition free_ports (ip : ip_address) (ports : gset port) :=
+    own aneris_freeports_name (◯ ({[ ip := (GSet ports)]})).
 
-Lemma mapsto_node_agree `{distG Σ} n γs γs' :
-  n n↦ γs -∗ n n↦ γs' -∗ ⌜γs = γs'⌝.
-Proof.
-  apply wand_intro_r.
-  rewrite /ownS mapsto_node_eq -own_op own_valid discrete_valid.
-  f_equiv=> /auth_frag_proj_valid /=. rewrite singleton_op singleton_valid.
-  apply (agree_op_invL' (A := node_gnamesO)).
-Qed.
+End definitions.
 
-Lemma node_in_map `{distG Σ} n γ's (m : gmap ip_address node_gnames) :
-  ⊢ (n n↦ γ's -∗ ownS dist_map_name m -∗ ⌜m !! n = Some γ's⌝)%I.
-Proof.
-  iIntros "H1 H2".
-  iCombine "H2" "H1" as "H".
-  rewrite /ownS mapsto_node_eq -own_op own_valid.
-  iDestruct "H" as %HvalidR. iPureIntro.
-  revert HvalidR.
-  rewrite auth_both_valid.
-  rewrite singleton_included_l=> -[[y [Hlookup Hless]] Hvalid].
-  assert (Hvalidy := lookup_valid_Some _ n y Hvalid Hlookup).
-  revert Hlookup.
-  rewrite lookup_fmap fmap_Some_equiv=> -[v' [Hl Heq]]. revert Hless Heq.
-  rewrite Some_included_total.
-  destruct (to_agree_uninj y Hvalidy) as [y' <-].
-  rewrite to_agree_included.
-  intros Heq Heq'%(to_agree_inj y' v').
-  apply leibniz_equiv in Heq.
-  apply leibniz_equiv in Heq'.
-    by simplify_eq.
-Qed.
+(** Heap points-to (LaTeX: [\mapsto]) *)
+Notation "l ↦[ ip ]{ q } v" := (mapsto_heap ip l q v)
+  (at level 20, q at level 50, format "l  ↦[ ip ]{ q }  v") : bi_scope.
+Notation "l ↦[ ip ] v" := (l ↦[ip]{1} v)%I
+  (at level 20, format "l  ↦[ ip ]  v") : bi_scope.
+Notation "l ↦[ ip ]{ q } -" := (∃ v, l ↦[ip]{q} v)%I
+  (at level 20, q at level 50, format "l  ↦[ ip ]{ q }  -") : bi_scope.
+Notation "l ↦[ ip ] -" := (l ↦[ip]{1} -)%I
+  (at level 20, format "l  ↦[ ip ]  -") : bi_scope.
 
-Global Instance mapsto_s_fractional `{distG Σ} (n : ip_address) h q z :
-  AsFractional (mapsto_s n h q z) (λ q, mapsto_s n h q z) q.
-Proof.
-  constructor; first trivial. intros p p'. rewrite /mapsto_s. iSplit.
-  - iDestruct 1 as (?) "[#? Hmap]".
-    iDestruct (fractional_split with "Hmap") as "[Hmap Hmap']".
-    iSplitL "Hmap"; iExists _; eauto.
-  - iDestruct 1 as "[Hmap Hmap']". iDestruct "Hmap" as (?) "[#Hn1 Hmap]".
-    iDestruct "Hmap'" as (?) "[#Hn2 Hmap']".
-    iDestruct (mapsto_node_agree with "Hn1 Hn2") as %->.
-    iExists _. iFrame "#"; iFrame.
-Qed.
+(** Socket points-to (LaTeX: [\hookrightarrow]) *)
+Notation "z ↪[ ip ]{ q } s" := (mapsto_socket ip z q s)
+  (at level 20, q at level 50, format "z  ↪[ ip ]{ q }  s") : bi_scope.
+Notation "z ↪[ ip ] s" := (z ↪[ ip ]{1} s)%I (at level 20) : bi_scope.
 
-Definition IsNode `{distG Σ} n := (∃ γs, n n↦ γs)%I.
-Global Instance IsNode_persistent `{distG Σ} n : Persistent (IsNode n).
-Proof. apply _. Qed.
-
-Lemma exists_IsNode `{distG Σ} n γs : n n↦ γs -∗ IsNode n.
-Proof. iIntros "?". by iExists _. Qed.
-
-Global Opaque IsNode.
-
-(** Fixed socket end-points in the system *)
-
-Definition Fixed `{distG Σ} A := ownF A.
-
-Lemma ownF_agree `{distG Σ} A B : Fixed A -∗ Fixed B -∗ ⌜A = B⌝.
-Proof.
-  iIntros "HA HB".
-  by iDestruct (own_valid_2 with "HA HB") as %?%agree_op_invL'.
-Qed.
-
-(** Socket interpretations a ⤇ Φ *)
-
-Global Instance saved_pred_proper `{savedPredG Σ A} n γ:
-  Proper ((dist n) ==> (dist n)) (@saved_pred_own Σ A _ γ : (A -d> iPropO Σ) -d> iPropO Σ).
-Proof.
-  intros Φ Ψ Hps.
-  f_equiv.
-  destruct n; first done.
-    by apply dist_S.
-Qed.
-
-Global Instance saved_pred_proper' `{savedPredG Σ A} γ:
-  Proper ((≡) ==> (≡)) (@saved_pred_own Σ A _ γ : (A -d> iPropO Σ) -d> iPropO Σ).
-Proof.
-  apply ne_proper => n. apply _.
-Qed.
-
-Definition si_pred `{distG Σ} a (Φ : socket_interp Σ) : iProp Σ :=
-  (∃ γ, a γ↦ γ ∗ saved_pred_own γ Φ)%I.
-
-Global Instance si_pred_prop `{distG Σ} a : Proper ((≡) ==> (≡)) (si_pred a).
-Proof.
-  intros x y Heq.
-  apply exist_proper => z; f_equiv.
-  by rewrite Heq.
-Qed.
-
+(** Socket inteerpretation (LaTeX: [\Mapsto]) *)
 Notation "a ⤇ Φ" := (si_pred a Φ) (at level 20).
 
-(** Free IP addresses *)
+Lemma node_gnames_auth_init `{anerisPreG Σ} :
+  ⊢ |==> ∃ γ, own (A:=authR node_gnames_mapUR) γ (● (to_agree <$> ∅)).
+Proof. apply own_alloc. by apply auth_auth_valid. Qed.
 
-Definition FreeIPs_ctx `{distG Σ} (F : gset ip_address) :=
-  own dist_freeips_name (● GSet F).
+Lemma saved_si_init `{anerisPreG Σ} :
+  ⊢ |==> ∃ γ, own (A := authR socket_interpUR) γ (● (to_agree <$> ∅) ⋅ ◯ (to_agree <$> ∅)).
+Proof. apply own_alloc. by apply auth_both_valid. Qed.
 
-Definition FreeIP `{distG Σ} (ip : ip_address) :=
-  own dist_freeips_name (◯ GSet {[ ip ]}).
-
-Lemma is_FreeIP `{distG Σ} F ip :
-  FreeIPs_ctx F -∗ FreeIP ip -∗ ⌜ip ∈ F⌝.
-Proof.
-  iIntros "HF Hip". iDestruct (own_valid_2 with "HF Hip") as %[_ Hi].
-  iPureIntro.
-  move: (Hi 0%nat). rewrite /= left_id.
-  move => [? [/to_agree_injN /discrete /leibniz_equiv_iff <- [/gset_disj_included ? _]]].
-  by apply elem_of_subseteq_singleton.
+Lemma saved_si_update `{anerisG Σ} (A : gset socket_address) γsi f :
+  ⊢ own (A := authR socket_interpUR) γsi (● (to_agree <$> ∅)) ∗
+    own (A := authR socket_interpUR) γsi (◯ (to_agree <$> ∅)) ==∗
+    ∃ M : gmap socket_address gname,
+      ⌜elements (dom (gset socket_address) M) ≡ₚ elements A⌝ ∗
+       own (A:=authR socket_interpUR) γsi (● (to_agree <$> M)) ∗
+       [∗ map] a ↦ γ ∈ M, own (A:=authR socket_interpUR)
+                              γsi (◯ {[ a := (to_agree γ) ]}) ∗
+                              saved_pred_own (A:=message) γ (f a).
+  iIntros "[Hsi Hsi']".
+  pose proof (NoDup_elements A) as Hnd.
+  iInduction (elements A) as [|a l] "IHl" forall "Hsi Hsi'".
+   - iModIntro. iExists ∅.
+     rewrite big_sepM_empty fmap_empty; iFrame.
+     iPureIntro. by rewrite dom_empty_L.
+   - inversion Hnd as [|? ? ? Hrd']; subst.
+     iMod ("IHl" $! Hrd' with "Hsi Hsi'") as (M HMl) "[HM HML]"; iFrame.
+     iMod (saved_pred_alloc (f a)) as (γ) "Hγ".
+     assert (a ∉ dom (gset _) M) as Hnm.
+     { by rewrite -elem_of_elements HMl. }
+     iMod (own_update (A:=authR socket_interpUR) _ _
+                      (● (<[a := to_agree γ]>(to_agree <$> M)) ⋅
+                         (◯ ({[a := to_agree γ]}))) with "HM") as "[HM Hγ']".
+     { apply auth_update_alloc. rewrite -insert_empty.
+       rewrite /ε /= /gmap_unit. apply alloc_local_update; [|done].
+       apply not_elem_of_dom. by rewrite dom_fmap. }
+     iModIntro.
+     iExists (<[a:= γ]> M).
+     rewrite !fmap_insert; iFrame.
+     rewrite big_sepM_insert; [|by apply not_elem_of_dom].
+     iFrame. iPureIntro.
+     rewrite dom_insert_L elements_union_singleton //. auto.
 Qed.
 
-Lemma Use_FreeIP `{distG Σ} F ip :
-  FreeIPs_ctx F -∗ FreeIP ip ==∗ FreeIPs_ctx (F ∖ {[ ip ]}).
-Proof.
-  iIntros "HF Hip".
-  iDestruct (is_FreeIP with "HF Hip") as %Hip.
-  replace F with ({[ ip ]} ∪ (F ∖ {[ ip ]})) at 1; last first.
-  { rewrite (comm_L _ {[ _ ]}) difference_union_L
-    -(comm_L _ {[ _ ]}) subseteq_union_1_L //.
-    by apply elem_of_subseteq_singleton. }
-  iCombine "HF" "Hip" as "H".
-  iMod (own_update with "H") as "H"; last by iFrame "H".
-  apply auth_update_dealloc.
-  rewrite -gset_disj_union; last by set_solver.
-  by apply gset_disj_dealloc_empty_local_update.
-Qed.
+Lemma fixed_init `{anerisPreG Σ} A :
+  ⊢ |==> ∃ γ, own (A := agreeR (gsetUR socket_address)) γ (to_agree A).
+Proof. by apply own_alloc. Qed.
 
-Lemma FreeIps_alloc `{inG Σ (authUR (gset_disjUR ip_address))}
-      (F : gset ip_address) :
-  ⊢ |==> ∃ γ, own γ (● GSet F) ∗ [∗ set] ip ∈ F, own γ (◯ GSet {[ ip ]}).
+Lemma free_ports_auth_init `{anerisPreG Σ} :
+  ⊢ |==> ∃ γ, own (A:=authUR (gmapUR ip_address (gset_disjUR port))) γ (● ∅).
+Proof. apply own_alloc. by apply auth_auth_valid. Qed.
+
+Lemma free_ips_init `{anerisPreG Σ} A :
+  ⊢ |==> ∃ γ, own γ (● GSet A) ∗ [∗ set] ip ∈ A, own γ (◯ GSet {[ ip ]}).
 Proof.
-  iMod (own_alloc (● GSet ∅)) as (γ) "HM"; first by apply auth_auth_valid.
+  iMod (own_alloc (● GSet ∅)) as (γ) "HM"; [by apply auth_auth_valid|].
   iAssert (|==>
              ∃ M : gset ip_address,
-               (⌜elements M ≡ₚ elements F⌝)
+               (⌜elements M ≡ₚ elements A⌝)
                  ∗ own γ (● GSet M) ∗ [∗ set] ip ∈ M, own γ (◯ GSet {[ ip ]}))%I
     with "[HM]" as "HF".
-  { pose proof (NoDup_elements F) as Hnd.
-    iInduction (elements F) as [|a l] "IHl".
+  { pose proof (NoDup_elements A) as Hnd.
+    iInduction (elements A) as [|a l] "IHl".
     - iModIntro. iExists ∅.
       rewrite big_sepS_empty. iFrame.
-      by iPureIntro.
+        by iPureIntro.
     - inversion Hnd as [|? ? ? Hrd']; subst.
       iMod ("IHl" $! Hrd' with "HM") as (M HMl) "[HM HML]"; iFrame.
       assert (a ∉ M) as Hnm.
       { by rewrite -elem_of_elements HMl. }
       iMod (own_update _ _ (● GSet ({[a]} ∪ M) ⋅ ◯ GSet {[a]}) with "HM")
         as "[HM Ha]".
-      { apply auth_update_alloc.
-        apply gset_disj_alloc_empty_local_update; last by set_solver. }
+      { apply auth_update_alloc, gset_disj_alloc_empty_local_update.
+        set_solver. }
       iModIntro.
       iExists ({[a]} ∪ M); iFrame.
       iSplit; first by iPureIntro; rewrite elements_union_singleton // HMl.
-      rewrite big_sepS_insert; last done. iFrame. }
+      rewrite big_sepS_insert //. iFrame. }
   iMod "HF" as (M HMF) "[? ?]".
-  replace M  with F; first by iModIntro; iExists _; iFrame.
+  replace M with A; first by iModIntro; iExists _; iFrame.
   apply elem_of_equiv_L => x.
-  rewrite -!elem_of_elements.
-  rewrite -elem_of_list_permutation_proper; eauto.
+  rewrite -!elem_of_elements -elem_of_list_permutation_proper; eauto.
 Qed.
 
-Definition FreePorts_ctx `{distG Σ} (P : gmap ip_address (gset_disjUR port)) :=
-  own dist_freeports_name (● P).
+Section resource_lemmas.
+  Context `{aG : !anerisG Σ}.
 
-Definition FreePorts `{distG Σ} (ip : ip_address) (ports : gset port) :=
-  own dist_freeports_name (◯ ({[ ip := (GSet ports)]})).
+  Global Instance mapsto_node_persistent ip γn : Persistent (mapsto_node ip γn).
+  Proof. rewrite mapsto_node_eq /mapsto_node_def. apply _. Qed.
+  Global Instance mapsto_node_timeless ip γn : Timeless (mapsto_node ip γn).
+  Proof. rewrite mapsto_node_eq /mapsto_node_def. apply _. Qed.
 
-Lemma FreePorts_included `{distG Σ} P ip ports :
-  FreePorts_ctx P -∗ FreePorts ip ports -∗
+  Global Instance is_node_persistent ip : Persistent (is_node ip).
+  Proof. apply _. Qed.
+
+  Lemma mapsto_node_agree ip γn γn' :
+    mapsto_node ip γn -∗ mapsto_node ip γn' -∗ ⌜γn = γn'⌝.
+  Proof.
+    apply wand_intro_r.
+    rewrite /node_gnames_auth mapsto_node_eq -own_op own_valid discrete_valid.
+    f_equiv=> /auth_frag_proj_valid /=. rewrite singleton_op singleton_valid.
+    apply (agree_op_invL' (A := node_gnamesO)).
+  Qed.
+
+  Lemma node_gnames_valid ip γn m :
+   node_gnames_auth m -∗ mapsto_node ip γn -∗ ⌜m !! ip = Some γn⌝.
+  Proof.
+    iIntros "H1 H2".
+    iCombine "H2" "H1" as "H".
+    rewrite /node_gnames_auth mapsto_node_eq -own_op own_valid.
+    iDestruct "H" as %HvalidR. iPureIntro.
+    revert HvalidR.
+    rewrite comm auth_both_valid.
+    rewrite singleton_included_l=> -[[y [Hlookup Hless]] Hvalid].
+    assert (Hvalidy := lookup_valid_Some _ ip y Hvalid Hlookup).
+    revert Hlookup.
+    rewrite lookup_fmap fmap_Some_equiv=> -[v' [Hl Heq]]. revert Hless Heq.
+    rewrite Some_included_total.
+    destruct (to_agree_uninj y Hvalidy) as [y' <-].
+    rewrite to_agree_included.
+    intros Heq%leibniz_equiv Heq'%(to_agree_inj y' v')%leibniz_equiv.
+    by simplify_eq.
+  Qed.
+
+  Lemma node_gnames_alloc γn m ip :
+    m !! ip = None →
+    node_gnames_auth m ==∗ node_gnames_auth (<[ip:=γn]> m) ∗ mapsto_node ip γn.
+  Proof.
+    iIntros (?) "Hm". rewrite mapsto_node_eq /mapsto_node_def.
+    iMod (own_update _ _
+                     (● (to_agree <$> (<[ip:=γn]> m)) ⋅ (◯ {[ ip := to_agree γn ]})
+                      : authR node_gnames_mapUR) with "Hm") as "[Hm Hn]".
+    { rewrite fmap_insert. eapply auth_update_alloc.
+      apply (alloc_singleton_local_update (A := (agreeR node_gnamesO))); last done.
+      rewrite -not_elem_of_dom dom_fmap_L not_elem_of_dom //. }
+    iModIntro. iFrame.
+  Qed.
+
+  Global Instance mapsto_heap_timeless l ip q v :
+    Timeless (l ↦[ip]{q} v).
+  Proof. apply _. Qed.
+  Global Instance mapsto_heap_fractional l ip v :
+    Fractional (λ q, l ↦[ip]{q} v)%I.
+  Proof.
+    rewrite /mapsto_heap /Fractional=> p q. iSplit.
+    - iDestruct 1 as (?) "[#? [H1 H2]]".
+      iSplitL "H1"; iExists _; eauto.
+    - iDestruct 1 as "[H1 H2]".
+      iDestruct "H1" as (?) "[Hn1 Hp]".
+      iDestruct "H2" as (?) "[Hn2 Hq]".
+      iDestruct (mapsto_node_agree with "Hn1 Hn2") as %->.
+      iExists _. iFrame.
+  Qed.
+  Global Instance mapsto_heap_as_fractional l ip q v :
+    AsFractional (l ↦[ip]{q} v) (λ q, l ↦[ip]{q} v)%I q.
+  Proof. split; [done|]. apply _. Qed.
+
+  Global Instance mapsto_socket_timeless z ip q s :
+    Timeless (z ↪[ ip ]{ q } s).
+  Proof.
+    rewrite /mapsto_socket /Timeless.
+    iIntros ">H". iDestruct "H" as (γn) "[H1 H2]".
+    iExists _. iFrame.
+  Qed.
+  Global Instance mapsto_socket_fractional z ip s :
+    Fractional (λ q, z ↪[ip]{q} s)%I.
+  Proof.
+    rewrite /mapsto_socket /Fractional=> p q. iSplit.
+    - iDestruct 1 as (?) "[#? [H1 H2]]".
+      iSplitL "H1"; iExists _; eauto.
+    - iDestruct 1 as "[H1 H2]".
+      iDestruct "H1" as (?) "[Hn1 Hp]".
+      iDestruct "H2" as (?) "[Hn2 Hq]".
+      iDestruct (mapsto_node_agree with "Hn1 Hn2") as %->.
+      iExists _. iFrame.
+  Qed.
+  Global Instance mapsto_socket_as_fractional z ip q s :
+    AsFractional (z ↦[ip]{q} s) (λ q, z ↦[ip]{q} s)%I q.
+  Proof. split; [done|]. apply _. Qed.
+
+  Lemma node_ctx_init σ s :
+    ⊢ |==> ∃ (γn : node_gnames), heap_ctx γn σ ∗ sockets_ctx γn s.
+  Proof.
+    iMod (gen_heap_light_init σ) as (γh) "Hh".
+    iMod (gen_heap_light_init s) as (γs) "Hs".
+    iExists {| heap_name := γh; sockets_name := γs |}.
+    iModIntro. iFrame.
+  Qed.
+
+  Lemma fixed_agree A B : fixed A -∗ fixed B -∗ ⌜A = B⌝.
+  Proof.
+    iIntros "HA HB".
+    by iDestruct (own_valid_2 with "HA HB") as %?%agree_op_invL'.
+  Qed.
+
+  Global Instance saved_pred_proper `{savedPredG Σ A} n γ:
+    Proper ((dist n) ==> (dist n))
+           (@saved_pred_own Σ A _ γ : (A -d> iPropO Σ) -d> iPropO Σ).
+  Proof.
+    intros Φ Ψ Hps.
+    f_equiv. destruct n; [done|].
+    by apply dist_S.
+  Qed.
+  Global Instance saved_pred_proper' `{savedPredG Σ A} γ:
+    Proper ((≡) ==> (≡)) (@saved_pred_own Σ A _ γ : (A -d> iPropO Σ) -d> iPropO Σ).
+  Proof. solve_proper. Qed.
+  Global Instance si_pred_prop `{anerisG Σ} a : Proper ((≡) ==> (≡)) (si_pred a).
+  Proof. solve_proper. Qed.
+
+  Lemma free_ip_included A ip :
+    free_ips_auth A -∗ free_ip ip -∗ ⌜ip ∈ A⌝.
+  Proof.
+    iIntros "HF Hip". iDestruct (own_valid_2 with "HF Hip") as %[_ Hi].
+    iPureIntro.
+    move: (Hi 0%nat). rewrite /= left_id.
+    move => [? [/to_agree_injN /discrete /leibniz_equiv_iff <- [/gset_disj_included ? _]]].
+    by apply elem_of_subseteq_singleton.
+  Qed.
+
+  Lemma free_ip_dealloc A ip :
+    free_ips_auth A -∗ free_ip ip ==∗ free_ips_auth (A ∖ {[ ip ]}).
+  Proof.
+    iIntros "HF Hip".
+    iDestruct (free_ip_included with "HF Hip") as %Hip.
+    replace A with ({[ ip ]} ∪ (A ∖ {[ ip ]})) at 1; last first.
+    { rewrite (comm_L _ {[ _ ]}) difference_union_L
+      -(comm_L _ {[ _ ]}) subseteq_union_1_L //.
+        by apply elem_of_subseteq_singleton. }
+    iCombine "HF" "Hip" as "H".
+    iMod (own_update with "H") as "H"; last by iFrame "H".
+    apply auth_update_dealloc.
+    rewrite -gset_disj_union; last by set_solver.
+      by apply gset_disj_dealloc_empty_local_update.
+  Qed.
+
+  Lemma free_ports_included P ip ports :
+    free_ports_auth P -∗
+    free_ports ip ports -∗
     ∃ ports', ⌜P !! ip = Some (GSet ports') ∧ ports ⊆ ports'⌝.
-Proof.
-  iIntros "HP Hip"; rewrite /FreePorts_ctx /FreePorts.
-  iDestruct (own_valid_2 with "HP Hip") as
-      %[[y [Hy1%leibniz_equiv Hy2]]%singleton_included_l Hv]%auth_both_valid.
-  iPureIntro.
-  revert Hy2; rewrite Some_included_total.
-  destruct y as [ports'|].
-  - eexists; split; first by rewrite Hy1.
-    by apply gset_disj_included.
-  - by specialize (Hv ip); rewrite Hy1 in Hv.
-Qed.
+  Proof.
+    iIntros "HP Hip"; rewrite /free_ports_auth /free_ports.
+    iDestruct (own_valid_2 with "HP Hip") as
+        %[[y [Hy1%leibniz_equiv Hy2]]%singleton_included_l Hv]%auth_both_valid.
+    iPureIntro.
+    revert Hy2; rewrite Some_included_total.
+    destruct y as [ports'|].
+    - eexists; split; first by rewrite Hy1.
+      by apply gset_disj_included.
+    - by specialize (Hv ip); rewrite Hy1 in Hv.
+  Qed.
 
-Lemma FreePorts_distribute `{distG Σ} ip ports ports' :
-  ports ## ports' →
-  FreePorts ip (ports ∪ ports') ⊣⊢ FreePorts ip ports ∗ FreePorts ip ports'.
-Proof.
-  intros ?.
-  by rewrite /FreePorts -gset_disj_union // -own_op -auth_frag_op singleton_op.
-Qed.
+  Lemma free_ports_split ip ports ports' :
+    ports ## ports' →
+    free_ports ip (ports ∪ ports') ⊣⊢ free_ports ip ports ∗ free_ports ip ports'.
+  Proof.
+    intros ?.
+    by rewrite /free_ports -gset_disj_union //
+       -own_op -auth_frag_op singleton_op.
+  Qed.
 
-Lemma FreePorts_alloc `{distG Σ} P ip ports :
-  ip ∉ (dom (gset _) P) →
-  FreePorts_ctx P ==∗ FreePorts_ctx (<[ ip := GSet ports ]>P) ∗ FreePorts ip ports.
-Proof.
-  iIntros (?) "HP"; rewrite /FreePorts_ctx /FreePorts.
-  iMod (own_update _ _ (● _ ⋅ ◯ {[ ip := (GSet ports)]}) with "HP")
-    as "[HP Hip]"; last by iFrame.
-  apply auth_update_alloc, alloc_singleton_local_update; last done.
-  by eapply (not_elem_of_dom (D := gset ip_address)).
-Qed.
+  Lemma free_ports_alloc P ip ports :
+    ip ∉ (dom (gset _) P) →
+    free_ports_auth P ==∗
+    free_ports_auth (<[ ip := GSet ports ]>P) ∗ free_ports ip ports.
+  Proof.
+    iIntros (?) "HP"; rewrite /free_ports_auth /free_ports.
+    iMod (own_update _ _ (● _ ⋅ ◯ {[ ip := (GSet ports)]}) with "HP")
+      as "[HP Hip]"; last by iFrame.
+    apply auth_update_alloc, alloc_singleton_local_update; last done.
+    by eapply (not_elem_of_dom (D := gset ip_address)).
+  Qed.
 
-Lemma FreePorts_dealloc `{distG Σ} P ip ports :
-  FreePorts_ctx P -∗ FreePorts ip ports ==∗
+  Lemma free_ports_dealloc P ip ports :
+    free_ports_auth P -∗
+    free_ports ip ports ==∗
     ∃ ports', ⌜P !! ip = Some (GSet ports') ∧ ports ⊆ ports'⌝ ∗
-      FreePorts_ctx (<[ip := GSet (ports' ∖ ports)]> P).
-Proof.
-  iIntros "HP Hip"; rewrite /FreePorts_ctx /FreePorts.
-  iDestruct (FreePorts_included with "HP Hip") as (ports') "[% %]".
-  iMod (own_update_2 _ _ _
-          (● <[ip := GSet (ports' ∖ ports)]>P ⋅
-           ◯ <[ ip := GSet ∅ ]>{[ ip := (GSet ports)]}) with "HP Hip")
-    as "[? ?]".
-  { apply auth_update.
-    eapply insert_local_update;
-      [done|eapply (lookup_singleton (M := gmap _))|].
-    apply gset_disj_dealloc_local_update. }
-  by iExists _; iFrame.
-Qed.
+              free_ports_auth (<[ip := GSet (ports' ∖ ports)]> P).
+  Proof.
+    iIntros "HP Hip".
+    iDestruct (free_ports_included with "HP Hip") as (ports') "[% %]".
+    iMod (own_update_2 _ _ _
+      (● <[ip := GSet (ports' ∖ ports)]>P ⋅ ◯ <[ ip := GSet ∅ ]>{[ ip := (GSet ports)]})
+            with "HP Hip")
+      as "[? ?]".
+    { apply auth_update.
+      eapply insert_local_update; [done|eapply (lookup_singleton (M := gmap _))|].
+      apply gset_disj_dealloc_local_update. }
+      by iExists _; iFrame.
+  Qed.
 
-(** Definitions for the global state invariant *)
+  Lemma socket_interp_alloc a φ sis:
+    sis !! a = None →
+    saved_si_auth sis ==∗
+    ∃ γsi, saved_si_auth (<[a:=γsi]>sis) ∗ a ⤇ φ.
+  Proof.
+    iIntros (Hnone) "Hsi".
+    iMod (saved_pred_alloc φ) as (γsi) "#Hsipred".
+    iMod (own_update _ _
+            (● (to_agree <$> (<[a:=γsi]> sis)) ⋅ (◯ {[ a := to_agree γsi ]})
+             : authR socket_interpUR) with "Hsi") as "[Hsi #sip]".
+    { rewrite fmap_insert.
+      apply auth_update_alloc, alloc_singleton_local_update; [|done].
+      rewrite lookup_fmap Hnone //. }
+    iModIntro. iExists _. iFrame. iExists _. iFrame "#".
+  Qed.
 
-Definition gnames_coherence (γmap : gmap ip_address node_gnames)
-           (heaps : gmap ip_address heap) (sockets : gmap ip_address sockets) :=
-  dom (gset ip_address) γmap = dom (gset ip_address) heaps ∧
-  dom (gset ip_address) γmap = dom (gset ip_address) sockets.
+  Lemma socket_interp_agree a Φ Ψ x :
+    a ⤇ Φ -∗ a ⤇ Ψ -∗ ▷ (Φ x ≡ Ψ x).
+  Proof.
+    iIntros "#H1 #H2".
+    iDestruct "H1" as (γ) "[H1 H1']".
+    iDestruct "H2" as (γ') "[H2 H2']".
+    iDestruct (own_valid_2 with "H1 H2") as %Hvalid.
+    rewrite -auth_frag_op singleton_op in Hvalid.
+    apply singleton_valid in Hvalid.
+    apply (agree_op_invL' γ γ') in Hvalid.
+    rewrite Hvalid.
+    iDestruct (saved_pred_agree _ _ _ x with "H1' H2'") as "H".
+    iExact "H".
+  Qed.
 
-Definition IPs (P : ports_in_use) := dom (gset ip_address) P.
+  Lemma socket_interp_pred_equiv a Φ Ψ :
+    a ⤇ Φ -∗ a ⤇ Ψ -∗ ▷ (Φ ≡ Ψ).
+  Proof.
+    iIntros "#H1 #H2".
+    iDestruct "H1" as (γ) "[H1 H1']".
+    iDestruct "H2" as (γ') "[H2 H2']".
+    iDestruct (own_valid_2 with "H1 H2") as %Hvalid.
+    rewrite -auth_frag_op singleton_op in Hvalid.
+    apply singleton_valid in Hvalid.
+    apply (agree_op_invL' γ γ') in Hvalid.
+    rewrite Hvalid discrete_fun_equivI. iIntros (?).
+    by iDestruct (saved_pred_agree with "H1' H2'") as "H".
+  Qed.
 
-(* Addresses with interpretations are bound. *)
-Definition socket_interp_coherence `{distG Σ} (P : ports_in_use) :=
-  (∃ si A,
-    (* the addresses in A are also in the domain of ips *)
-    ⌜∀ a, a ∈ A → ip_of_address a ∈ IPs P⌝ ∗
-    (* for all addresses in the system, being in si means either having a
-       Fixed interpretation (a ∈ A) or being dynamically bound. *)
-    ⌜∀ a, (ip_of_address a ∈ IPs P) →
-      (a ∈ dom (gset socket_address) si ↔
-       a ∈ A ∨ (a ∉ A ∧ ∀ ps, P !! ip_of_address a = Some ps → port_of_address a ∈ ps))⌝ ∗
-      Fixed A ∗
-      own (A:=socket_interpR) dist_si_name (● si) ∗
-      ([∗ set] s ∈ (dom (gset socket_address) si), ∃ φ, s ⤇ φ))%I.
-
-(* The local state of each node *)
-Definition local_state_interp `{distG Σ}
-      (σ : state) (ip : ip_address) (x : node_gnames) :=
-  (∃ (h : heap) (Sn : sockets),
-      (* there should be a heap *)
-      ⌜state_heaps σ !! ip = Some h⌝ ∗
-      (* there should be a socket map *)
-      ⌜state_sockets σ !! ip = Some Sn⌝ ∗
-      (* its a valid node *)
-      ip n↦ x ∗
-      (* the state owns the authoritative part of the heaps *)
-      gen_heap_ctx (hG := gen_heap_loc_instance (heap_name x) (heap_meta_name x)) h ∗
-      gen_heap_ctx (hG := gen_heap_soc_instance (socket_name x) (socket_meta_name x)) Sn ∗
-     (* we own half of the resource for all the sockets to disallow
-       'fabricating' receiving messages *)
-      ([∗ map] h↦s ∈ Sn, h s↦[ip]{1/2} s)
-  )%I.
-
-(* The ports of all bound addresses are in ips *)
-Definition bound_ports_coherence (S : sockets) (Piu : ports_in_use) :=
-  ∀ h s a P R T, S !! h = Some (s, R, T) →
-               saddress s = Some a →
-               Piu !! ip_of_address a = Some P →
-               (port_of_address a) ∈ P.
-
-Definition socket_handlers_coherence (Sn : sockets)  :=
-  ∀ h h' s s' R R' T T',
-    Sn !! h = Some (s, R, T) →
-    Sn !! h' = Some (s', R', T') →
-    is_Some (saddress s) → saddress s' = saddress s →
-    h' = h.
-
-(* Received messages at a socket are in the message soup *)
-Definition socket_messages_coherence (Sn : sockets) (M : message_soup) :=
-  ∀ h s R T a,
-    Sn !! h = Some (s, R, T) →
-    saddress s = Some a →
-     (∀ m, m ∈ R → m_destination m = a ∧ m ∈ M) ∧
-     (∀ m, m ∈ T → m_sender m = a ∧ m ∈ M).
-
-(* ips adresses of each nodes are disjoint *)
-Definition socket_addresses_coherence (Sn: sockets) (ip: ip_address) :=
-  ∀ h s R T a,
-    Sn !! h = Some (s, R, T) →
-    saddress s = Some a →
-    ip_of_address a = ip.
-
-Definition network_sockets_coherence
-    (S : gmap ip_address sockets) M P :=
-  ∀ (ip : ip_address) (Sn : sockets),
-    S !! ip = Some Sn →
-    (* the network should be coherent wrt. to the node n *)
-    bound_ports_coherence Sn P ∧
-    socket_handlers_coherence Sn ∧
-    (* the messages received should be coherent wrt. to node n *)
-    socket_messages_coherence Sn M ∧
-    socket_addresses_coherence Sn ip.
-
- Definition message_received_at `{distG Σ}
-   (S : gmap ip_address sockets) (m : message) (a: socket_address) :=
-   ∃ Sn h s R T,
-     S !! (ip_of_address a) = Some Sn ∧
-     Sn !! h = Some (s, R, T) ∧
-     saddress s = Some a ∧
-     m ∈ R.
-
-Definition message_received `{distG Σ} (S : gmap ip_address sockets) (m : message) :=
-  ∃ a, message_received_at S m a.
-
-Definition network_messages_coherence
-           `{distG Σ} (S : gmap ip_address sockets) (M : message_soup) :=
-  ([∗ set] m ∈ M,
-   (* either m is governed by a protocol and the network owns the resources *)
-     (∃ (Φ : socket_interp Σ), (m_destination m) ⤇ Φ ∗ ▷ Φ m) ∨
-   (* or m has been delivered *)
-     ⌜message_received S m⌝)%I.
-
-Definition network_coherence `{distG Σ} S M P :=
-  (⌜network_sockets_coherence S M P⌝ ∗ network_messages_coherence S M)%I.
-
-Definition FipPiu `{distG Σ} σ :=
-  (∃ Fip Piu, (⌜dom (gset _) Piu ## Fip ∧
-               (∀ ip, ip ∈ Fip → state_ports_in_use σ !! ip = Some ∅) ∧
-               (∀ ip, ip ∈ Fip → state_heaps σ !! ip = None ∧
-                                 state_sockets σ !! ip = None) ∧
-               (∀ ip P, Piu !! ip = Some (GSet P) →
-                        ∃ Q, (state_ports_in_use σ) !! ip = Some Q ∧ P ## Q )⌝)
-                ∗ FreeIPs_ctx Fip ∗ FreePorts_ctx Piu)%I.
-
-(* global state interpretation *)
-Global Instance distG_irisG `{distG Σ} :
-  irisG aneris_lang Σ :=
-  {|
-    iris_invG := _;
-    state_interp σ κ _ :=
-      (
-        ∃ (m : gmap ip_address node_gnames),
-          ⌜gnames_coherence m (state_heaps σ) (state_sockets σ)⌝ ∗
-           socket_interp_coherence (state_ports_in_use σ) ∗
-           ownS dist_map_name m ∗
-           ([∗ map] n ↦ γs ∈ m, local_state_interp σ n γs) ∗
-           FipPiu σ ∗
-           network_coherence
-           (state_sockets σ) (state_ms σ) (state_ports_in_use σ)
-      )%I;
-    fork_post _ := True%I;
-  |}.
-
-Global Opaque iris_invG.
+End resource_lemmas.
