theories/aneris_lang/basic_lifting.v
@@ -1,3 +1,0 @@
-From aneris.aneris_lang Require Export lifting_pure.
-From aneris.aneris_lang Require Export lifting_network_local.
-From aneris.aneris_lang Require Export lifting_network_aware.
