theories/aneris_lang/lib/network_helpers.v
@@ -5,11 +5,11 @@ From aneris.aneris_lang.lib Require Import assert.
 
 Section code.
 
-  Definition unSOME : ground_lang.val :=
+  Definition unSOME : base_lang.val :=
     λ: "p",
     match: "p" with NONE => assert #false | SOME "p'" => "p'" end.
 
-  Definition listen : ground_lang.val :=
+  Definition listen : base_lang.val :=
     (
       rec: "loop" "socket" "handle" :=
         match: ReceiveFrom "socket" with
@@ -19,7 +19,7 @@ Section code.
         end
     )%V.
 
-  Definition listen_wait : ground_lang.val :=
+  Definition listen_wait : base_lang.val :=
     (
       rec: "loop" "socket" :=
         match: ReceiveFrom "socket" with
@@ -40,7 +40,7 @@ Import uPred.
 
 
 Section library.
-  Context `{dG : distG Σ}.
+  Context `{dG : anerisG Σ}.
 
   Lemma unSOME_spec ip v v' :
     {{{ ⌜v = SOMEV v'⌝ }}} unSOME (Val v) @[ip] {{{ RET v'; True }}}.
@@ -54,19 +54,19 @@ Section library.
     saddress s = Some a →
     (∀ m,
       {{{ ⌜m_destination m = a⌝ ∗ P ∗
-          ((⌜m ∉ R⌝ ∗ h s↦[ip]{1/2} (s, {[m]} ∪ R, T) ∗ φ m) ∨
-          (⌜m ∈ R⌝ ∗ h s↦[ip]{1/2} (s, R, T)))
+          ((⌜m ∉ R⌝ ∗ h ↪[ip] (s, {[m]} ∪ R, T) ∗ φ m) ∨
+          (⌜m ∈ R⌝ ∗ h ↪[ip] (s, R, T)))
       }}}
          (Val handler) #(m_body m) #(m_sender m) @[ip]
       {{{ v, RET v; Q v }}}) -∗
-      {{{ P ∗ h s↦[ip]{1/2} (s, R, T) ∗ a ⤇ φ }}}
+      {{{ P ∗ h ↪[ip] (s, R, T) ∗ a ⤇ φ }}}
          listen #(LitSocket h) (Val handler) @[ip]
       {{{ v, RET v; Q v }}}.
   Proof.
      iIntros (n Haddr) "#Hhandler". iLöb as "IH".
-     iAlways. iIntros (Φ) "(HP & Hsocket & #Hsi) HΦ".
+     iModIntro. iIntros (Φ) "(HP & Hsocket & #Hsi) HΦ".
      wp_rec. wp_let. rewrite /n. wp_bind (ReceiveFrom _).
-     wp_apply (aneris_wp_receive_from_2 with "[$]"); [done|done|].
+     wp_apply (aneris_wp_receivefrom_alt with "[$]"); [done|done|].
      iIntros (r) "[(-> & Hs) | Hrd ]"; simpl.
      - wp_pures. iApply ("IH" with "[-HΦ]"); by iFrame.
      - iDestruct "Hrd" as (m Hdst ->) "[ (% & Hs & Hφ) | (% & Hs) ]"; wp_pures;
@@ -76,16 +76,16 @@ Section library.
   Lemma listen_wait_spec ip h s R T a φ :
     ip = ip_of_address a →
     saddress s = Some a →
-  {{{ h s↦[ip]{1/2} (s, R, T) ∗ a ⤇ φ}}}
+  {{{ h ↪[ip] (s, R, T) ∗ a ⤇ φ}}}
      listen_wait #(LitSocket h) @[ip]
   {{{ m, RET (#(m_body m), #(m_sender m));
-      ((⌜m ∉ R⌝ ∗ h s↦[ip]{1/2} (s, {[ m ]} ∪ R, T) ∗ a ⤇ φ ∗ ▷ φ m) ∨
-       ⌜m ∈ R⌝ ∗ h s↦[ip]{1/2} (s, R, T))
+      ((⌜m ∉ R⌝ ∗ h ↪[ip] (s, {[ m ]} ∪ R, T) ∗ a ⤇ φ ∗ ▷ φ m) ∨
+       ⌜m ∈ R⌝ ∗ h ↪[ip] (s, R, T))
   }}}.
   Proof.
     iIntros (n Haddr Φ) "(Hs & #Hsi) HΦ".
     iLöb as "IH". wp_rec.
-    wp_apply (aneris_wp_receive_from_2 with "[$Hs]");
+    wp_apply (aneris_wp_receivefrom_alt with "[$Hs]");
       [done|done|by iFrame "#"|].
     iIntros (r)  "[(-> & Hs) | Hrd ]"; simpl; wp_pures.
     - by iApply ("IH" with "Hs HΦ").
