theories/aneris_lang/lib/nodepar.v
@@ -1,33 +1,32 @@
 From iris.base_logic.lib Require Export invariants.
 From iris.proofmode Require Import tactics.
 From iris.algebra Require Import excl.
-From aneris.aneris_lang Require Export lang lifting network notation tactics proofmode.
+From aneris.aneris_lang Require Export lang tactics proofmode.
 Set Default Proof Using "Type".
 
-Notation "( n1 ; ip1 ; e1 ) ||| ( n2 ; ip2 ; e2 )" :=
-  (Start n2 ip2 e2, Start n1 ip1 e1)%E.
+Notation "( ip1 ; e1 )  ||| ( ip2 ; e2 )" :=
+  (Start ip2 e2, Start ip1 e1)%E.
 
 Section proof.
-  Context `{ppd : !pingpongG Σ}
-          `{dG : !distG Σ}.
+  Context `{dG : !anerisG Σ}.
 
-  Lemma par_spec Φ1 Φ2 P1 P2 n1 n2 ip1 ip2 e1 e2 :
-    n1 ≠ "system" ∧ n2 ≠ "system" →
+  Lemma par_spec Φ1 Φ2 P1 P2 ip1 ip2 e1 e2 :
+    ip1 ≠ "system" ∧ ip2 ≠ "system" →
     Φ1 ∗ Φ2 ∗
-    FreeIP ip1 ∗ FreeIP ip2 ∗
-    ((IsNode n1 -∗ Φ1 -∗ FreePorts ip1 P1 -∗ WP ⟨n1;e1⟩ {{ _, True }}) ∗
-     (isNode n2 -∗ Φ2 -∗ FreePorts ip2 P2 -∗ WP ⟨n2;e2⟩ {{ _, True }}))%I ⊢
-    WP ⟨"system"; (n1; ip1; e1) ||| (n2; ip2; e2)⟩ {{ _, True }}.
+    free_ip ip1 ∗ free_ip ip2 ∗
+    ((Φ1 -∗ free_ports ip1 P1 -∗ WP e1 @[ip1] {{ _, True }}) ∗
+     (Φ2 -∗ free_ports ip2 P2 -∗ WP e2 @[ip2] {{ _, True }}))%I ⊢
+    WP ((ip1; e1) ||| (ip2; e2)) @["system"] {{ _, True }}.
   Proof.
     iIntros ([Hn1 Hn2]) "(HΦ1 & HΦ2 & HIP1 & HIP2 & Hwp1 & Hwp2)".
-    wp_apply (wp_start with "[-]"); first auto. iFrame.
+    wp_apply (aneris_wp_start with "[-]"); first auto. iFrame.
     iSplitR "HΦ1 Hwp1"; last first.
-    { iNext. iIntros "Hn Hp". iApply ("Hwp1" with "Hn HΦ1 Hp"). }
+    { iNext. iIntros "Hp". iApply ("Hwp1" with "HΦ1 Hp"). }
     iNext. simpl.
-    wp_apply (wp_start with "[-]"); first auto. iFrame.
+    wp_apply (aneris_wp_start with "[-]"); first auto. iFrame.
     iSplitR "HΦ2 Hwp2"; last first.
-    { iNext. iIntros "Hn Hp". iApply ("Hwp2" with "Hn HΦ2 Hp"). }
-    iNext. simpl. by wp_pures.
+    { iNext. iIntros "Hp". iApply ("Hwp2" with "HΦ2 Hp"). }
+    iNext. by wp_pures.
   Qed.
 
 End proof.
