theories/aneris_lang/lifting.v
@@ -1,0 +1,558 @@
+From stdpp Require Import fin_maps gmap.
+From iris.bi.lib Require Import fractional.
+From iris.program_logic Require Export weakestpre lifting.
+From iris.program_logic Require Import ectx_lifting total_ectx_lifting.
+From iris.proofmode Require Import tactics.
+From aneris.aneris_lang Require Import aneris_lang base_lang state_interp.
+From RecordUpdate Require Import RecordSet.
+Set Default Proof Using "Type".
+
+Import uPred.
+Import Network.
+Import RecordSetNotations.
+
+(** The tactic [inv_head_step] performs inversion on hypotheses of the shape
+    [head_step]. The tactic will discharge head-reductions starting from values, and
+    simplifies hypothesis related to conversions from and to values, and finite map
+    operations. This tactic is slightly ad-hoc and tuned for proving our lifting
+    lemmas. *)
+Ltac inv_head_step :=
+  repeat
+    match goal with
+    | _ => progress simplify_map_eq/= (* simplify memory stuff *)
+    | H : aneris_to_val _ = Some _ |- _ => apply to_base_aneris_val in H
+    | H : base_lang.head_step ?e _ _ _ _ _ |- _ =>
+      try (is_var e; fail 1); (* inversion yields many goals if [e] is a variable
+     and can thus better be avoided. *)
+      inversion H; subst; clear H
+    | H : head_step ?e _ _ _ _ _ |- _ =>
+      try (is_var e; fail 1);
+      inversion H; subst; clear H
+    | H: socket_step _ ?e _ _ _ _ _ _ _ |- _ =>
+      try (is_var e; fail 1);
+      inversion H; subst; clear H
+    end.
+
+Local Ltac solve_exec_safe :=
+  intros;
+  repeat match goal with
+         | H: _ ∧ _ |- _ => destruct H as [??]
+         end;
+  simplify_eq;
+  do 3 eexists; eapply (LocalStepPureS _ ∅); econstructor; eauto.
+Local Ltac solve_exec_puredet :=
+  simpl; intros; inv_head_step;
+  first (by repeat match goal with
+                   | H: _ ∧ _ |- _ => destruct H as [??]; simplify_eq
+                   | H : to_val _ = Some _ |- _ =>
+                     rewrite to_of_val in H; simplify_eq
+                   end);
+  try by match goal with
+         | H : socket_step _ _ _ _ _ _ _ _ _ |- _ =>
+           inversion H
+         end.
+Local Ltac solve_pure_exec :=
+  simplify_eq; rewrite /PureExec; intros;
+  apply nsteps_once, pure_head_step_pure_step;
+  constructor; [solve_exec_safe | solve_exec_puredet].
+
+Local Hint Constructors head_step : core.
+Local Hint Resolve alloc_fresh : core.
+Local Hint Resolve to_of_val : core.
+
+Instance into_val_val n v : IntoVal (mkExpr n (Val v)) (mkVal n v).
+Proof. done. Qed.
+Instance as_val_val n v : AsVal (mkExpr n (Val v)).
+Proof. by exists (mkVal n v). Qed.
+
+Instance into_val_base_val v : IntoVal (Val v) v.
+Proof. done. Qed.
+Instance as_val_base_val v : AsVal (Val v).
+Proof. by exists v. Qed.
+
+Local Ltac solve_atomic :=
+  apply strongly_atomic_atomic, ectx_language_atomic;
+    [inversion 1; inv_head_step; naive_solver
+    |apply ectxi_language_sub_redexes_are_values; intros [] **; inv_head_step;
+       rewrite /aneris_to_val /is_Some /=; eexists; by
+         match goal with
+         | H: _ = _ |- _ => rewrite -H
+         end
+    ].
+
+Lemma aneris_base_fill K ip e :
+  mkExpr ip (fill (Λ := base_ectxi_lang) K e) =
+  fill (Λ := aneris_ectxi_lang) K (mkExpr ip e).
+Proof.
+  revert e; induction K as [|k K IHK] using rev_ind; first done.
+  intros e.
+  rewrite !fill_app /= -IHK /=; done.
+Qed.
+
+Instance aneris_pure_exec_fill
+         (K : list ectx_item) ip (φ : Prop) (n : nat) (e1 e2 : expr) :
+  PureExec φ n (mkExpr ip e1) (mkExpr ip e2) →
+  @PureExec aneris_lang φ n
+            (mkExpr ip (@fill base_ectxi_lang K e1))
+            (mkExpr ip (@fill base_ectxi_lang K e2)).
+Proof.
+  intros.
+  rewrite !aneris_base_fill.
+  eapply pure_exec_ctx; first apply _; done.
+Qed.
+
+Instance binop_atomic n s op v1 v2 :
+  Atomic s (mkExpr n (BinOp op (Val v1) (Val v2))).
+Proof. solve_atomic. Qed.
+Instance alloc_atomic n s v : Atomic s (mkExpr n (Alloc (Val v))).
+Proof. solve_atomic. Qed.
+Instance load_atomic n s v : Atomic s (mkExpr n (Load (Val v))).
+Proof. solve_atomic. Qed.
+Instance store_atomic n s v1 v2 : Atomic s (mkExpr n (Store (Val v1) (Val v2))).
+Proof. solve_atomic. Qed.
+Instance cmpxchg_atomic n s v0 v1 v2 :
+  Atomic s (mkExpr n (CAS (Val v0) (Val v1) (Val v2))).
+Proof. solve_atomic. Qed.
+Instance fork_atomic n s e : Atomic s (mkExpr n (Fork e)).
+Proof. solve_atomic. Qed.
+Instance skip_atomic n s : Atomic s (mkExpr n Skip).
+Proof. solve_atomic. Qed.
+
+Instance newsocket_atomic n v0 v1 v2 s :
+  Atomic s (mkExpr n  (NewSocket (Val v0) (Val v1) (Val v2))).
+Proof. solve_atomic. Qed.
+Instance socketbind_atomic n v0 v1  s :
+  Atomic s (mkExpr n (SocketBind (Val v0) (Val v1))).
+Proof. solve_atomic. Qed.
+Instance sendto_atomic n v0 v1 v2 s :
+  Atomic s (mkExpr n (SendTo (Val v0) (Val v1) (Val v2))).
+Proof. solve_atomic. Qed.
+Instance receivefrom_atomic n v s : Atomic s (mkExpr n (ReceiveFrom (Val v))).
+Proof. solve_atomic. Qed.
+
+Class AsRecV (v : val) (f x : binder) (erec : expr) :=
+  as_recv : v = RecV f x erec.
+Hint Mode AsRecV ! - - - : typeclass_instances.
+Definition AsRecV_recv f x e : AsRecV (RecV f x e) f x e := eq_refl.
+Hint Extern 0 (AsRecV (RecV _ _ _) _ _ _) =>
+  apply AsRecV_recv : typeclass_instances.
+
+Instance pure_rec f x (erec : expr) :
+  PureExec True 1 (mkExpr n (Rec f x erec)) (mkExpr n (Val $ RecV f x erec)).
+Proof. solve_pure_exec. Qed.
+Instance pure_pairc (v1 v2 : val) :
+  PureExec True 1 (mkExpr n (Pair (Val v1) (Val v2))) (mkExpr n (Val $ PairV v1 v2)).
+Proof. solve_pure_exec. Qed.
+Instance pure_injlc (v : val) :
+  PureExec True 1 (mkExpr n (InjL $ Val v)) (mkExpr n (Val $ InjLV v)).
+Proof. solve_pure_exec. Qed.
+Instance pure_injrc (v : val) :
+  PureExec True 1 (mkExpr n (InjR $ Val v)) (mkExpr n (Val $ InjRV v)).
+Proof. solve_pure_exec. Qed.
+
+Instance pure_beta f x erec (v1 v2 : val) `{!AsRecV v1 f x erec} :
+  PureExec True 1 (mkExpr n (App (Val v1) (Val v2)))
+           (mkExpr n (subst' x v2 (subst' f v1 erec))).
+Proof. unfold AsRecV in *. solve_pure_exec. Qed.
+
+Instance pure_unop op v v' :
+  PureExec (un_op_eval op v = Some v') 1 (mkExpr n (UnOp op (Val v)))
+           (mkExpr n (of_val v')).
+Proof. solve_pure_exec. Qed.
+
+Instance pure_binop op v1 v2 v' :
+  PureExec (bin_op_eval op v1 v2 = Some v') 1
+           (mkExpr n (BinOp op (Val v1) (Val v2))) (mkExpr n (of_val v')).
+Proof. solve_pure_exec. Qed.
+
+Instance pure_if_true e1 e2 :
+  PureExec True 1 (mkExpr n (If (Val $ LitV $ LitBool true) e1 e2)) (mkExpr n e1).
+Proof. solve_pure_exec. Qed.
+
+Instance pure_if_false e1 e2 :
+  PureExec True 1 (mkExpr n (If (Val $ LitV $ LitBool false) e1 e2))
+           (mkExpr n e2).
+Proof. solve_pure_exec. Qed.
+
+Instance pure_fst v1 v2  :
+  PureExec True 1 (mkExpr n (Fst (PairV v1 v2))) (mkExpr n (Val v1)).
+Proof. solve_pure_exec. Qed.
+
+Instance pure_snd v1 v2  :
+  PureExec True 1 (mkExpr n (Snd (PairV v1 v2))) (mkExpr n (Val v2)).
+Proof. solve_pure_exec. Qed.
+
+Instance pure_find_from v0 v1 n1 v2 v' :
+  PureExec (index n1 v2 v0 = v' ∧ Z.of_nat n1 = v1) 1
+           (mkExpr n (FindFrom (Val $ LitV $ LitString v0)
+                       (Val $ LitV $ LitInt v1)
+                       (Val $ LitV $ LitString v2)))
+           (mkExpr n (base_lang.of_val (option_nat_to_val v'))).
+Proof. solve_pure_exec. Qed.
+
+Instance pure_substring v0 v1 n1 v2 n2 v' :
+  PureExec (substring n1 n2 v0 = v' ∧ Z.of_nat n1 = v1 ∧ Z.of_nat n2 = v2) 1
+           (mkExpr
+              n (Substring
+                   (LitV $ LitString v0) (LitV $ LitInt v1) (LitV $ LitInt v2)))
+           (mkExpr n (base_lang.of_val (LitV $ LitString v'))).
+Proof. solve_pure_exec. Qed.
+
+Instance pure_case_inl v e1 e2  :
+  PureExec True 1 (mkExpr n (Case (Val $ InjLV v) e1 e2))
+           (mkExpr n (App e1 (Val v))).
+Proof. solve_pure_exec. Qed.
+
+Instance pure_case_inr v e1 e2 :
+  PureExec True 1 (mkExpr n (Case (Val $ InjRV v) e1 e2))
+           (mkExpr n (App e2 (Val v))).
+Proof. solve_pure_exec. Qed.
+
+Instance pure_make_address v1 v2 :
+  PureExec True 1
+           (mkExpr n (MakeAddress (LitV (LitString v1)) (LitV (LitInt (v2)))))
+           (mkExpr
+              n (LitV (LitSocketAddress (SocketAddressInet v1 (Z.to_pos v2))))).
+Proof. solve_pure_exec. Qed.
+
+Opaque aneris_state_interp.
+
+Section primitive_laws.
+  Context `{anerisG Σ}.
+
+  Implicit Types P Q : iProp Σ.
+  Implicit Types Φ : aneris_val → iProp Σ.
+  Implicit Types v : val.
+  Implicit Types e : expr.
+  Implicit Types σ : state.
+  Implicit Types M R T : message_soup.
+  Implicit Types m : message.
+  Implicit Types A B : gset socket_address.
+  Implicit Types a : socket_address.
+  Implicit Types ip : ip_address.
+  Implicit Types sh : socket_handle.
+  Implicit Types skt : socket.
+
+  Lemma wp_fork n k E e Φ :
+    ▷ Φ (mkVal n #()) ∗ ▷ WP (mkExpr n e) @ k; ⊤ {{ _, True }} ⊢
+    WP (mkExpr n (Fork e)) @ k; E {{ Φ }}.
+  Proof.
+    iIntros "[HΦ He]". iApply wp_lift_atomic_head_step; [done|].
+    iIntros (σ1 κ κs m) "Hσ !>". iSplit.
+    - iPureIntro. eexists; solve_exec_safe.
+    - iIntros (? ? ? ?). inv_head_step. iFrame. done.
+  Qed.
+
+  Lemma wp_alloc n k E v :
+    {{{ ▷ is_node n }}}
+      (mkExpr n (Alloc (Val v))) @ k; E
+    {{{ l, RET (mkVal n #l); l ↦[n] v }}}.
+  Proof.
+    iIntros (Φ) ">Hn HΦ".
+    iApply wp_lift_atomic_head_step_no_fork; auto.
+    iIntros (σ ? ? ?) "Hσ !> /=".
+    iDestruct (is_node_heap_valid with "Hσ Hn") as (h) "%".
+    iSplitR.
+    { iPureIntro. do 4 eexists. eapply LocalStepS; eauto. }
+    iIntros (v2 σ2 efs Hstep); inv_head_step.
+    iSplitR; [done|]. iModIntro.
+    iMod (aneris_state_interp_alloc_heap with "Hn Hσ") as "[Hσ Hl]"; [done..|].
+    iModIntro. iFrame.
+    by iApply "HΦ".
+  Qed.
+
+  Lemma wp_load n k E l q v :
+    {{{ ▷ l ↦[n]{q} v }}}
+      (mkExpr n (Load #l)) @ k; E
+    {{{ RET (mkVal n v); l ↦[n]{q} v }}}.
+  Proof.
+    iIntros (Φ) ">Hl HΦ".
+    iApply wp_lift_atomic_head_step_no_fork; auto.
+    iIntros (σ κ κs n') "Hσ !> /=".
+    iDestruct (aneris_state_interp_heap_valid with "Hσ Hl") as (h) "[% %]".
+    iSplit.
+    { iPureIntro. do 4 eexists. eapply LocalStepS; eauto. eapply LoadS; eauto. }
+    iIntros (e2 σ2 efs Hstep). inv_head_step.
+    rewrite insert_id //. destruct σ; iFrame.
+    do 2 iModIntro. iSplit; [done|]. by iApply "HΦ".
+  Qed.
+
+  Lemma wp_store n k E l v1 v2 :
+    {{{ ▷ l ↦[n] v1 }}}
+      (mkExpr n (Store #l (Val v2))) @ k; E
+    {{{ RET (mkVal n #()); l ↦[n] v2 }}}.
+  Proof.
+    iIntros (Φ) ">Hl HΦ". iApply wp_lift_atomic_head_step_no_fork; auto.
+    iIntros (σ κ κs n') "Hσ !>".
+    iDestruct (aneris_state_interp_heap_valid with "Hσ Hl") as (h) "[% %]".
+    iSplit.
+    { iPureIntro; do 4 eexists. eapply LocalStepS; eauto. econstructor. }
+    iIntros (????); inv_head_step. iModIntro.
+    iMod (aneris_state_interp_heap_update with "[$Hσ $Hl]") as "[Hσ Hl]";
+      [done|].
+    iModIntro. iSplit; [done|]. iFrame. by iApply "HΦ".
+  Qed.
+
+  Lemma wp_cas_fail n k E l q v v1 v2 :
+    v ≠ v1 →
+    {{{ ▷ l ↦[n]{q} v }}}
+      (mkExpr n (CAS #l (Val v1) (Val v2))) @ k; E
+    {{{ RET (mkVal n #false); l ↦[n]{q} v }}}.
+  Proof.
+    iIntros (Heq Φ) ">Hl HΦ".
+    iApply wp_lift_atomic_head_step_no_fork; auto.
+    iIntros (σ κ κs n') "Hσ !>".
+    iDestruct (aneris_state_interp_heap_valid with "Hσ Hl") as (h) "[% %]".
+    iSplit.
+    { iPureIntro; do 4 eexists. eapply LocalStepS; eauto. by econstructor. }
+    iIntros (????); inv_head_step. iModIntro.
+    rewrite insert_id //. destruct σ; iFrame.
+    iModIntro. iSplit; [done|]. by iApply "HΦ".
+  Qed.
+
+  Lemma wp_cas_suc n k E l v1 v2 :
+    {{{ ▷ l ↦[n] v1 }}}
+      (mkExpr n (CAS #l (Val v1) (Val v2))) @ k; E
+    {{{ RET (mkVal n #true); l ↦[n] v2 }}}.
+  Proof.
+    iIntros (Φ) ">Hl HΦ". iApply wp_lift_atomic_head_step_no_fork; auto.
+    iIntros (σ κ κs n') "Hσ !>".
+    iDestruct (aneris_state_interp_heap_valid with "Hσ Hl") as (h) "[% %]".
+    iSplit.
+    { iPureIntro; do 4 eexists. eapply LocalStepS; eauto. by econstructor. }
+    iIntros (????); inv_head_step. iModIntro.
+    iMod (aneris_state_interp_heap_update with "[$Hσ $Hl]") as "[Hσ Hl]";
+      [done|].
+    iModIntro. iSplit; [done|]. iFrame. by iApply "HΦ".
+  Qed.
+
+  Lemma wp_start ip ports k E e Φ :
+    ip ≠ "system" →
+    ▷ free_ip ip ∗
+    ▷ Φ (mkVal "system" #()) ∗
+    ▷ (is_node ip -∗ free_ports ip ports -∗
+               WP (mkExpr ip e) @ k; ⊤ {{ _, True }})
+    ⊢ WP (mkExpr "system" (Start (LitString ip) e)) @ k; E {{ Φ }}.
+  Proof.
+    iIntros (?) "(>Hfip & HΦ & Hwp)".
+    iApply (wp_lift_head_step with "[-]"); first auto.
+    iIntros (σ κ κs n) "Hσ".
+    iMod (fupd_intro_mask _ ∅ True%I with "[]") as "Hmk"; first set_solver; auto.
+    iDestruct (aneris_state_interp_free_ip_valid with "Hσ Hfip") as "(% & % & %)".
+    iModIntro; iSplit.
+    { iPureIntro. do 4 eexists. apply (AssignNewIpStepS _ _ []); eauto. }
+    iNext. iIntros (e2 σ2 efs Hrd). iMod "Hmk" as "_".
+    inv_head_step.
+    iMod (aneris_state_interp_alloc_node with "[$]") as "(Hn & Hports & Hσ)".
+    iModIntro. iFrame.
+    iSplitL "HΦ"; [by iApply wp_value|].
+    iSplitL; [|done].
+    by iApply ("Hwp" with "[$] [$]").
+  Qed.
+
+  Lemma wp_new_socket ip s E f t p :
+    {{{ ▷ is_node ip }}}
+      (mkExpr ip (NewSocket (Val $ LitV $ LitAddressFamily f)
+                            (Val $ LitV $ LitSocketType t)
+                            (Val $ LitV $ LitProtocol p))) @ s; E
+    {{{ sh, RET (mkVal ip (LitV (LitSocket sh)));
+          sh ↪[ip] ((mkSocket f t p None), ∅, ∅) }}}.
+  Proof.
+    iIntros (Φ) ">Hn HΦ".
+    iApply wp_lift_atomic_head_step_no_fork; first auto.
+    iIntros (σ κ κs n) "Hσ !> /=".
+    iDestruct (is_node_valid_sockets with "Hσ Hn") as (?) "%".
+    iSplitR.
+    { iPureIntro; do 4 eexists. eapply (SocketStepS _ _ _ _ _ _ _ _ []); eauto.
+      apply newsocket_fresh. }
+    set (sock := {| sfamily := f; stype := t; sprotocol := p; saddress := None |}).
+    iIntros (v2' ? ? Hstep) "!>"; inv_head_step.
+    iMod (aneris_state_interp_alloc_socket sock with "Hn Hσ") as "[Hσ Hsh]"; try done.
+    iModIntro. iFrame. iSplitR; [done|]. by iApply "HΦ".
+  Qed.
+
+  Lemma wp_socketbind_static s A E sh skt a:
+    saddress skt = None →
+    a ∈ A →
+    {{{ fixed A ∗
+        ▷ free_ports (ip_of_address a) {[port_of_address a]} ∗
+        ▷ sh ↪[ip_of_address a] (skt, ∅, ∅) }}}
+      (mkExpr (ip_of_address a)
+              (SocketBind (Val $ LitV $ LitSocket sh)
+                          (Val $ LitV $ LitSocketAddress a))) @ s; E
+   {{{ RET (mkVal (ip_of_address a) #0);
+         sh ↪[ip_of_address a] (skt<| saddress := Some a |>, ∅, ∅) ∗
+         ∃ φ, a ⤇ φ }}}.
+  Proof.
+    iIntros (?? Φ) "(#Hfixed & >Hp & >Hsh) HΦ".
+    iApply wp_lift_atomic_head_step_no_fork; first auto.
+    iIntros (σ κ κs n) "Hσ /=".
+    iDestruct (aneris_state_interp_socket_valid with "Hσ Hsh") as (?) "[% %]".
+    iDestruct (aneris_state_interp_free_ports_valid with "Hσ Hp") as (?) "[% %]".
+    iModIntro. iSplitR.
+    { iPureIntro; do 4 eexists. eapply (SocketStepS _ _ _ _ _ _ _ _ []); eauto.
+      by econstructor. }
+    iIntros (v2' ? ? Hstep) "!>"; inv_head_step.
+    iMod (aneris_state_interp_socketbind_static with "Hσ Hfixed Hsh Hp")
+      as "(Hσ & Hsh & Hφ)"; [done..|].
+    iModIntro. iSplitR; [done|]. iFrame.
+    iApply ("HΦ" with "[$]").
+  Qed.
+
+  Lemma wp_socketbind_dynamic skt A E sh k a φ :
+    saddress skt = None →
+    a ∉ A →
+    {{{ ▷ fixed A ∗
+        ▷ free_ports (ip_of_address a) {[port_of_address a]} ∗
+        ▷ sh ↪[ip_of_address a] (skt, ∅, ∅) }}}
+      (mkExpr (ip_of_address a)
+              (SocketBind (Val $ LitV $ LitSocket sh)
+                          (Val $ LitV $ LitSocketAddress a))) @ k; E
+    {{{ RET (mkVal (ip_of_address a) #0);
+          sh ↪[ip_of_address a] (skt <| saddress := Some a |>, ∅, ∅) ∗
+          a ⤇ φ }}}.
+  Proof.
+    iIntros (?? Φ) "(#>Hfixed & >Hp & >Hsh) HΦ".
+    iApply wp_lift_atomic_head_step_no_fork; first auto.
+    iIntros (σ κ κs n) "Hσ /=".
+    iDestruct (aneris_state_interp_socket_valid with "Hσ Hsh") as (?) "[% %]".
+    iDestruct (aneris_state_interp_free_ports_valid with "Hσ Hp") as (?) "[% %]".
+    iModIntro. iSplitR.
+    { iPureIntro; do 4 eexists. eapply (SocketStepS _ _ _ _ _ _ _ _ []); eauto.
+      by econstructor. }
+    iIntros (v2' ? ? Hstep) "!>"; inv_head_step.
+    iMod (aneris_state_interp_socketbind_dynamic with "Hσ Hfixed Hsh Hp")
+      as "(Hσ & Hsh & Hφ)"; [done..|].
+    iModIntro. iSplitR; [done|]. iFrame.
+    iApply ("HΦ" with "[$]").
+  Qed.
+
+  Lemma wp_send φ mbody sh skt a to k E R T:
+    let msg := mkMessage a to (sprotocol skt) mbody  in
+    saddress skt = Some a ->
+    {{{ ▷ sh ↪[ip_of_address a] (skt, R, T) ∗
+        ▷ to ⤇ φ ∗
+        ▷ φ msg }}}
+      (mkExpr (ip_of_address a)
+              (SendTo (Val $ LitV $ LitSocket sh) #mbody #to)) @ k; E
+    {{{ RET (mkVal (ip_of_address a) #(String.length mbody));
+          sh ↪[ip_of_address a] (skt, R, {[ msg ]} ∪ T) }}}.
+  Proof.
+    iIntros (? Hsome Φ) "(>Hsh & #Hφ & Hm) HΦ".
+    iApply wp_lift_atomic_head_step_no_fork; auto.
+    iIntros (σ κ κs n) "Hσ !>".
+    iDestruct (aneris_state_interp_socket_valid with "Hσ Hsh") as (?) "[% %]".
+    iSplitR.
+    { iPureIntro; do 4 eexists; eapply (SocketStepS _ _ _ _ _ _ _ _ []); eauto.
+        by econstructor. }
+    iIntros (????) "!>"; inv_head_step; rewrite -/msg.
+    iMod (aneris_state_interp_send with "Hsh Hφ Hm Hσ") as "[Hσ Hsh]";
+      [done..|].
+    iModIntro. iSplitR; [done|]. iFrame. by iApply "HΦ".
+  Qed.
+
+  Lemma wp_send_duplicate mbody sh skt a to k E R T:
+    let msg := mkMessage a to (sprotocol skt) mbody in
+    saddress skt = Some a ->
+    msg ∈ T →
+    {{{ ▷ sh ↪[ip_of_address a] (skt, R, T) }}}
+      (mkExpr (ip_of_address a)
+              (SendTo (Val $ LitV $ LitSocket sh) #mbody #to)) @ k; E
+    {{{ RET (mkVal (ip_of_address a) #(String.length mbody));
+        sh ↪[ip_of_address a] (skt, R, T) }}}.
+   Proof.
+    iIntros (msg Hsome Hmsg Φ) ">Hsh HΦ /=".
+    iApply wp_lift_atomic_head_step_no_fork; auto.
+    iIntros (σ κ κs n) "Hσ !>".
+    iDestruct (aneris_state_interp_socket_valid with "Hσ Hsh") as (?) "[% %]".
+    iSplitR.
+    { iPureIntro; do 4 eexists; eapply (SocketStepS _ _ _ _ _ _ _ _ []); eauto.
+        by econstructor. }
+    iIntros (????) "!>"; inv_head_step; rewrite -/msg.
+    iMod (aneris_state_interp_send_duplicate with "Hsh Hσ") as "[Hσ Hsh]";
+      [done..|].
+    iModIntro. iSplitR; [done|]. iFrame. by iApply "HΦ".
+   Qed.
+
+   Lemma wp_receivefrom_gen (Ψo : option (socket_interp Σ)) k a E sh skt R T :
+    saddress skt = Some a →
+    {{{ ▷ sh ↪[ip_of_address a] (skt, R, T) ∗
+          match Ψo with Some Ψ => a ⤇ Ψ | _ => True end }}}
+      (mkExpr (ip_of_address a)
+              (ReceiveFrom (Val $ LitV $ LitSocket sh))) @ k; E
+    {{{ r, RET (mkVal (ip_of_address a) r);
+        ((⌜r = NONEV⌝ ∗ sh ↪[ip_of_address a] (skt, R, T)) ∨
+        (∃ msg,
+          ⌜m_destination msg = a⌝ ∗
+          ⌜r = SOMEV (PairV (LitV $ LitString (m_body msg))
+                  (LitV $ LitSocketAddress (m_sender msg)))⌝ ∗
+          ((⌜msg ∉ R⌝ ∗ sh ↪[ip_of_address a] (skt, {[ msg ]} ∪ R, T) ∗
+             match Ψo with Some Ψ => Ψ msg | _ => ∃ φ, a ⤇ φ ∗ φ msg end) ∨
+            ⌜msg ∈ R⌝ ∗ sh ↪[ip_of_address a] (skt, R, T)))) }}}.
+  Proof.
+    iIntros (Hsome Φ) "[>Hsh #HΨ] HΦ /=".
+    iApply wp_lift_atomic_head_step_no_fork; auto.
+    iIntros (σ κ κs n) "Hσ !>".
+    iDestruct (aneris_state_interp_socket_valid with "Hσ Hsh") as (?) "[% %]".
+    iSplitR.
+    { iPureIntro; do 4 eexists; eapply (SocketStepS _ _ _ _ _ _ _ _ []); eauto.
+        by econstructor. }
+    iIntros (????); inv_head_step; (iSplitR; [done|]).
+    - (* received a message *)
+      iDestruct (aneris_state_interp_receive with "HΨ [$Hσ $Hsh]") as "H";
+        [done..|].
+      iDestruct "H" as (R') "[Hsi Hσ2]".
+      iNext. iMod "Hσ2" as "[$ Hsh]". iModIntro.
+      iApply "HΦ". iRight. iExists m. iFrame.
+      match goal with
+      | H: m ∈ messages_to_receive_at a (state_ms σ) |- _ =>
+        apply elem_of_filter in H as (? &?)
+      end.
+      do 2 (iSplit; [done|]).
+      iDestruct "Hsi" as "[(% & -> & ?) | (% & ->) ]"; [|eauto].
+      iLeft. by iFrame.
+    - (* did not receive a message *)
+      assert (<[ip_of_address a:=Sn']> (state_sockets σ) = state_sockets σ) as ->.
+      { by apply insert_id. }
+      iModIntro. iFrame. iApply "HΦ"; auto.
+  Qed.
+
+  Lemma wp_receivefrom k a E sh skt R T :
+    let ip := ip_of_address a in
+    saddress skt = Some a →
+    {{{ ▷ sh ↪[ip] (skt, R, T) }}}
+      (mkExpr ip (ReceiveFrom (Val $ LitV $ LitSocket sh))) @ k; E
+    {{{ r, RET (mkVal ip r);
+        ((⌜r = NONEV⌝ ∗ sh ↪[ip] (skt, R, T)) ∨
+        (∃ msg,
+          ⌜m_destination msg = a⌝ ∗
+          ⌜r = SOMEV (PairV (LitV $ LitString (m_body msg))
+                  (LitV $ LitSocketAddress (m_sender msg)))⌝ ∗
+          ((⌜msg ∉ R⌝ ∗ sh ↪[ip] (skt, {[ msg ]} ∪ R, T) ∗ ∃ φ, a ⤇ φ ∗ φ msg) ∨
+            ⌜msg ∈ R⌝ ∗ sh ↪[ip] (skt, R, T)))) }}}.
+   Proof.
+     iIntros (? Hs Φ) "Hsh HΦ".
+     iApply (wp_receivefrom_gen None with "[$]"); [done|].
+     iNext. iIntros (r) "Hr". iApply "HΦ"; eauto.
+   Qed.
+
+  Lemma wp_receivefrom_alt k a E sh skt R T φ :
+    let ip := ip_of_address a in
+    saddress skt = Some a →
+    {{{ ▷ sh ↪[ip] (skt, R, T) ∗ a ⤇ φ }}}
+      (mkExpr ip (ReceiveFrom (Val $ LitV $ LitSocket sh))) @ k; E
+    {{{ r, RET (mkVal ip r);
+        (⌜r = NONEV⌝ ∗ sh ↪[ip] (skt, R, T)) ∨
+        ∃ msg,
+          ⌜m_destination msg = a⌝ ∗
+          ⌜r = SOMEV (PairV (LitV $ LitString (m_body msg))
+                  (LitV $ LitSocketAddress (m_sender msg)))⌝ ∗
+          ((⌜msg ∉ R⌝ ∗ sh ↪[ip] (skt, {[ msg ]} ∪ R, T) ∗ φ msg) ∨
+            ⌜msg ∈ R⌝ ∗ sh ↪[ip] (skt, R, T)) }}}.
+   Proof.
+     iIntros (? Hs Φ) "Hsh HΦ".
+     iApply (wp_receivefrom_gen (Some φ) with "[$]"); [done|].
+     iNext. iIntros (r) "Hr". iApply "HΦ"; eauto.
+   Qed.
+
+End primitive_laws.
