theories/program_logic/gen_heap_light.v
@@ -1,0 +1,153 @@
+From iris.bi.lib Require Import fractional.
+From iris.proofmode Require Import tactics.
+From iris.algebra Require Import auth gmap frac agree.
+From iris.base_logic.lib Require Import gen_heap.
+From iris.base_logic.lib Require Export own.
+Set Default Proof Using "Type".
+Import uPred.
+
+Section definitions.
+  Context `{Countable L, hG : !inG Σ (authR (gen_heapUR L V))}.
+
+  Definition gen_heap_light_ctx (γ : gname) (σ : gmap L V) : iProp Σ :=
+    own γ (● (to_gen_heap σ)).
+
+  Definition lmapsto_def (γ : gname) (l : L) (q : Qp) (v: V) : iProp Σ :=
+    own γ (◯ {[ l := (q, to_agree (v : leibnizO V)) ]}).
+  Definition lmapsto_aux : seal (@lmapsto_def). Proof. by eexists. Qed.
+  Definition lmapsto := lmapsto_aux.(unseal).
+  Definition lmapsto_eq : @lmapsto = @lmapsto_def := lmapsto_aux.(seal_eq).
+End definitions.
+
+Local Notation "l ; γ ↦{ q } v" := (lmapsto γ l q v)
+  (at level 20, q at level 50, format "l  ;  γ  ↦{ q }  v") : bi_scope.
+Local Notation "l ; γ ↦ v" := (lmapsto γ l 1 v) (at level 20) : bi_scope.
+
+Local Notation "l ; γ ↦{ q } -" := (∃ v, l ; γ ↦{q} v)%I
+  (at level 20, q at level 50, format "l  ;  γ  ↦{ q }  -") : bi_scope.
+Local Notation "l ; γ ↦ -" := (l ; γ ↦{1} -)%I (at level 20) : bi_scope.
+
+Lemma gen_heap_light_init `{Countable L, !inG Σ (authR (gen_heapUR L V))} σ :
+  ⊢ |==> ∃ (γ : gname), gen_heap_light_ctx γ σ.
+Proof.
+  iMod (own_alloc (● to_gen_heap σ)) as (γ) "Hh".
+  { rewrite auth_auth_valid. exact: to_gen_heap_valid. }
+  eauto.
+Qed.
+
+Section gen_heap_light.
+  Context {L V} `{Countable L, !inG Σ (authR (gen_heapUR L V))}.
+  Implicit Types σ : gmap L V.
+  Implicit Types l : L.
+  Implicit Types v : V.
+
+  (** General properties of lmapsto *)
+  Global Instance lmapsto_timeless l γ q v : Timeless (l ; γ ↦{q} v).
+  Proof. rewrite lmapsto_eq /lmapsto_def. apply _. Qed.
+  Global Instance lmapsto_fractional l γ v : Fractional (λ q, l ; γ ↦{q} v)%I.
+  Proof.
+    intros p q. by rewrite lmapsto_eq /lmapsto_def -own_op -auth_frag_op
+      singleton_op -pair_op agree_idemp.
+  Qed.
+  Global Instance lmapsto_as_fractional l γ q v :
+    AsFractional (l ; γ ↦{q} v) (λ q, l ; γ ↦{q} v)%I q.
+  Proof. split; [done|]. apply _. Qed.
+
+  Lemma lmapsto_agree l γ q1 q2 v1 v2 :
+    l ; γ ↦{q1} v1 -∗ l ; γ ↦{q2} v2 -∗ ⌜v1 = v2⌝.
+  Proof.
+    apply wand_intro_r.
+    rewrite lmapsto_eq /lmapsto_def -own_op -auth_frag_op own_valid discrete_valid.
+    f_equiv. rewrite auth_frag_valid singleton_op singleton_valid -pair_op.
+    by intros [_ ?%agree_op_invL'].
+  Qed.
+
+  Lemma lmapsto_combine l γ q1 q2 v1 v2 :
+    l ; γ ↦{q1} v1 -∗ l ; γ ↦{q2} v2 -∗ l ; γ ↦{q1 + q2} v1 ∗ ⌜v1 = v2⌝.
+  Proof.
+    iIntros "Hl1 Hl2". iDestruct (lmapsto_agree with "Hl1 Hl2") as %->.
+    iCombine "Hl1 Hl2" as "Hl". eauto with iFrame.
+  Qed.
+
+  Global Instance ex_lmapsto_fractional l γ : Fractional (λ q, l ; γ ↦{q} -)%I.
+  Proof.
+    intros p q. iSplit.
+    - iDestruct 1 as (v) "[H1 H2]". iSplitL "H1"; eauto.
+    - iIntros "[H1 H2]". iDestruct "H1" as (v1) "H1". iDestruct "H2" as (v2) "H2".
+      iDestruct (lmapsto_agree with "H1 H2") as %->. iExists v2. by iFrame.
+  Qed.
+  Global Instance ex_lmapsto_as_fractional l γ q :
+    AsFractional (l ; γ ↦{q} -) (λ q, l ; γ ↦{q} -)%I q.
+  Proof. split; [done|]. apply _. Qed.
+
+  Lemma lmapsto_valid l γ q v : l ; γ ↦{q} v -∗ ✓ q.
+  Proof.
+    rewrite lmapsto_eq /lmapsto_def own_valid !discrete_valid -auth_frag_valid.
+    by apply pure_mono=> /singleton_valid [??].
+  Qed.
+  Lemma lmapsto_valid_2 l γ q1 q2 v1 v2 :
+    l ; γ ↦{q1} v1 -∗ l ; γ ↦{q2} v2 -∗ ✓ (q1 + q2)%Qp.
+  Proof.
+    iIntros "H1 H2". iDestruct (lmapsto_agree with "H1 H2") as %->.
+    iApply (lmapsto_valid l _ _ v2). by iFrame.
+  Qed.
+
+  Lemma lmapsto_lmapsto_ne l1 l2 γ q1 q2 v1 v2 :
+    ¬ ✓(q1 + q2)%Qp → l1 ; γ ↦{q1} v1 -∗ l2 ; γ ↦{q2} v2 -∗ ⌜l1 ≠ l2⌝.
+  Proof.
+    iIntros (?) "Hl1 Hl2"; iIntros (->).
+    by iDestruct (lmapsto_valid_2 with "Hl1 Hl2") as %?.
+  Qed.
+
+  (** Update lemmas *)
+  Lemma gen_heap_light_alloc σ l γ v :
+    σ !! l = None →
+    gen_heap_light_ctx γ σ ==∗ gen_heap_light_ctx γ (<[l:=v]>σ) ∗ l ; γ ↦ v.
+  Proof.
+    iIntros (Hσl). rewrite /gen_heap_light_ctx lmapsto_eq /lmapsto_def /=.
+    iIntros "Hσ".
+    iMod (own_update with "Hσ") as "[Hσ Hl]".
+    { eapply auth_update_alloc,
+        (alloc_singleton_local_update _ _ (1%Qp, to_agree (v:leibnizO _)))=> //.
+      by apply lookup_to_gen_heap_None. }
+    iModIntro.
+    rewrite to_gen_heap_insert. iFrame.
+  Qed.
+
+  Lemma gen_heap_light_alloc_gen σ σ' γ :
+    σ' ##ₘ σ →
+    gen_heap_light_ctx γ σ ==∗
+    gen_heap_light_ctx γ (σ' ∪ σ) ∗ ([∗ map] l ↦ v ∈ σ', l ; γ ↦ v).
+  Proof.
+    revert σ; induction σ' as [| l v σ' Hl IH] using map_ind; iIntros (σ Hdisj) "Hσ".
+    { rewrite left_id_L. auto. }
+    iMod (IH with "Hσ") as "[Hσ'σ Hσ']"; first by eapply map_disjoint_insert_l.
+    decompose_map_disjoint.
+    rewrite !big_opM_insert // -insert_union_l //.
+    by iMod (gen_heap_light_alloc with "Hσ'σ") as "($ & $ & $)";
+      first by apply lookup_union_None.
+  Qed.
+
+  Lemma gen_heap_light_valid σ l γ q v :
+    gen_heap_light_ctx γ σ -∗ l ; γ ↦{q} v -∗ ⌜σ !! l = Some v⌝.
+  Proof.
+    iIntros "Hσ Hl".
+    rewrite /gen_heap_light_ctx lmapsto_eq /lmapsto_def.
+    iDestruct (own_valid_2 with "Hσ Hl")
+      as %[Hl%gen_heap_singleton_included _]%auth_both_valid; auto.
+  Qed.
+
+  Lemma gen_heap_light_update γ σ l v1 v2 :
+    gen_heap_light_ctx γ σ -∗ l ; γ ↦ v1 ==∗
+    gen_heap_light_ctx γ (<[l:=v2]>σ) ∗ l ; γ ↦ v2.
+  Proof.
+    iIntros "Hσ Hl". rewrite /gen_heap_light_ctx lmapsto_eq /lmapsto_def.
+    iDestruct (own_valid_2 with "Hσ Hl")
+      as %[Hl%gen_heap_singleton_included _]%auth_both_valid.
+    iMod (own_update_2 with "Hσ Hl") as "[Hσ Hl]".
+    { eapply auth_update, singleton_local_update,
+        (exclusive_local_update _ (1%Qp, to_agree (v2:leibnizO _)))=> //.
+      by rewrite /to_gen_heap lookup_fmap Hl. }
+    iModIntro. iFrame "Hl". rewrite to_gen_heap_insert. iFrame.
+  Qed.
+End gen_heap_light.
